Started Assignment 2

Unification.thy
@@ -63,4 +63,85 @@ lemma var_term: "Var \<cdot> t = t"
 lemma Var_scomp [simp]: "Var \<circ>\<^sub>s \<sigma>= \<sigma>"
   by (auto simp add:var_term)
 
+fun sdom :: "('f,'v) subst \<Rightarrow> 'v set" where
+  "sdom \<sigma> = \<Union>x. \<sigma> x \<noteq> x"
+
+fun sran :: "('f,'v) subst \<Rightarrow> 'v set" where
+  "sran \<sigma> = set (map \<sigma> (sdom \<sigma>))"
+
+fun svran :: "('f,'v) subst \<Rightarrow> 'v set" where
+  "svran \<sigma> = (\<Union>t \<in> sran \<sigma>. fv t)" 
+
+lemma sdom_Var[simp]: "sdom Var = {}"
+  oops
+
+lemma svran_Var[simp]: "svran Var = {}"
+  oops
+
+lemma sdom_single_non_trivial[simp]: "t \<noteq> Var x \<Longrightarrow> sdom (Var (x:=t)) = {x}"
+  oops
+
+lemma svran_single_non_trivial[simp]: "t \<noteq> Var x \<Longrightarrow> svran (Var (x:=t)) = {x}"
+  oops
+
+lemma fv_apply_sdom_svran: "x \<in> (fv t - sdom \<sigma>) \<union> svran \<sigma>"
+  oops
+
+lemma sdom_scomp: "sdom (\<sigma> \<circ>\<^sub>s \<tau>) \<subseteq> sdom \<sigma> \<union> sdom \<tau>"
+  oops
+
+lemma svran_scomp: "svran (\<sigma> \<circ>\<^sub>s \<tau>) \<subseteq> svran \<sigma> \<union> svran \<tau>"
+  oops
+
+subsection \<open>Assignment 2\<close>
+
+type_synonym ('f,'v) equation = "('f,'v) term \<times> ('f,'v) term"
+
+type_synonym ('f,'v) system = "('f,'v) equation list"
+
+definition fv_eq :: "('f,'v) equation \<Rightarrow> 'v set" where
+  "fv_eq x = fv (fst x) \<union> fv (snd x)"
+
+definition sapply_eq :: "('f,'v) subst \<Rightarrow> ('f, 'v) equation \<Rightarrow> ('f,'v) equation"
+  where
+    "sapply_eq \<sigma> x = (sapply \<sigma> (fst x), sapply \<sigma> (snd x))"
+
+definition fv_sys :: "('f,'v) system \<Rightarrow> 'v set" where
+  "fv_sys x = Union (set (map fv_eq x))"
+
+definition sapply_sys :: "('f,'v) subst \<Rightarrow> ('f,'v) system \<Rightarrow> ('f,'v) system"
+  where
+  "sapply_sys \<sigma> x = map (sapply_eq \<sigma>) x"
+
+lemma fv_sapply_eq: "fv_eq (sapply_eq \<sigma> x) = (\<Union>x \<in> fv_eq x. fv (\<sigma> x))"
+  by (simp add: fv_eq_def sapply_eq_def fv_sapply)
+
+lemma fv_sapply_sys: "fv_sys (sapply_sys \<sigma> x) = (\<Union>x \<in> fv_sys x. fv (\<sigma> x))"
+  by (simp add: fv_sys_def sapply_sys_def fv_sapply_eq)
+
+lemma sapply_scomp_distrib_eq: "sapply_eq (\<sigma> \<circ>\<^sub>s \<tau> ) t = sapply_eq \<sigma> (sapply_eq \<tau>  t)"
+  by (simp add: sapply_eq_def sapply_scomp_distrib)
+
+lemma sapply_scomp_distrib_sys: "sapply_sys (\<sigma> \<circ>\<^sub>s \<tau> ) t = sapply_sys \<sigma> (sapply_sys \<tau>  t)"
+  by (simp add: sapply_sys_def sapply_scomp_distrib_eq)
+
+fun unifies :: "('f,'v) subst \<Rightarrow> ('f,'v) equation \<Rightarrow> bool"
+  where
+    "unifies \<sigma> (Var x, Var y) = (if \<sigma> x = \<sigma> y then True else False)"
+  | "unifies \<sigma> (Var x, Fun f xs) = False"
+  | "unifies \<sigma> (Fun f xs, Var y) = False"
+  | "unifies \<sigma> (x, y) = all (map (unifies \<sigma>) (\<sigma> \<cdot> x, \<sigma> \<cdot> y))"
+
+definition unifiess :: "('f,'v) subst \<Rightarrow> ('f,'v) system \<Rightarrow> bool" where
+  "unifiess \<sigma> x = all (map (unifies \<sigma>) x)"
+
+fun is_mgu :: "('f,'v) subst \<Rightarrow> ('f,'v) system \<Rightarrow> bool" where
+  "is_mgu \<sigma> x = True"
+
+lemma unifies_sapply_eq: "unifies \<sigma> (sapply_eq \<tau> eq) \<longleftrightarrow> unifies (\<sigma> \<circ>\<^sub>s \<tau>) eq"
+  oops
+
+lemma unifies_sapply_sys: "unifiess \<sigma> (sapply_sys \<tau> sys) \<longleftrightarrow> unifiess (\<sigma> \<circ>\<^sub>s \<tau>) sys"
+  oops
+
 end
